theories/ftlr/Seal.v
@@ -34,23 +34,24 @@ Section fundamental.
         fixpoint interp1 W (WSealRange p0 g0 b0 e0 a0) -∗
         fixpoint interp1 W (WSealed a0 sb).
   Proof.
-    iIntros (Hpseal Hwb) "#HVsb #HVsr".
-    rewrite (fixpoint_interp1_eq W (WSealRange _ _ _ _ _)) (fixpoint_interp1_eq W (WSealed _ _)) /= Hpseal /interp_sb.
-    iDestruct "HVsr" as "[Hss _]".
-    apply seq_between_dist_Some in Hwb.
-    iDestruct (big_sepL_delete with "Hss") as "[HSa0 _]"; eauto.
-    iDestruct "HSa0" as (P) "[% [HsealP HWcond]]".
-    iExists (P W).
-    repeat iSplitR; auto.
-    by iApply "HWcond".
-  Qed.
+    (* iIntros (Hpseal Hwb) "#HVsb #HVsr". *)
+    (* rewrite (fixpoint_interp1_eq W (WSealRange _ _ _ _ _)) (fixpoint_interp1_eq W (WSealed _ _)) /= Hpseal /interp_sb. *)
+    (* iDestruct "HVsr" as "[Hss _]". *)
+    (* apply seq_between_dist_Some in Hwb. *)
+    (* iDestruct (big_sepL_delete with "Hss") as "[HSa0 _]"; eauto. *)
+    (* iDestruct "HSa0" as (P) "[% [HsealP HWcond]]". *)
+    (* iExists (P W). *)
+    (* repeat iSplitR; auto. *)
+    (* by iApply "HWcond". *)
+  (* Qed. *)
+    Admitted.
 
   Lemma seal_case (W : WORLD) (regs : leibnizO Reg)
     (p p' : Perm) (g : Locality) (b e a : Addr)
     (w : Word) (ρ : region_type) (dst r1 r2 : RegName) (P:D):
     ftlr_instr W regs p p' g b e a w (Seal dst r1 r2) ρ P.
   Proof.
-    intros Hp Hsome i Hbae Hfp HO Hpers Hpwl Hregion Hnotrevoked Hnotfrozen Hi.
+    intros Hp Hsome HcorrectPC Hbae Hfp HO Hpers Hpwl Hregion Hnotrevoked Hnotfrozen Hi.
     iIntros "#IH #Hinv_interp #Hreg #Hinva #Hrcond #Hwcond #Hmono #HmonoV Hw Hsts Hown".
     iIntros "Hr Hstate Ha HPC Hmap".
     iInsert "Hmap" PC.
@@ -73,16 +74,16 @@ Section fundamental.
       { destruct (decide (PC = r1)); last auto. simplify_map_eq; auto. }
       rewrite lookup_insert_ne in Hr1; auto.
       iAssert (fixpoint interp1 W (WSealable sb)) as "#HVsb".
-      {
-        destruct (decide (r2 = PC)) as [Heq|Heq]; simplify_map_eq.
-        - rewrite (fixpoint_interp1_eq _ (WCap p g b e a)) /=.
-          destruct Hp as [Hp | [Hp | [Hp Hg] ] ]; subst p; try subst g.
-          all: iApply (big_sepL_mono with "Hinv_interp").
-          all: intros; iIntros "H"; simpl.
-          all: try( iDestruct "H"
-                   as (p P' Hfl HpersP') "(Hrel & Hzcond & Hrcond & Hwcond & HmonoR & %Hstate)").
-          all: iExists p,P'; iFrame "%∗".
-        - unshelve iSpecialize ("Hreg" $! r2 _ _ Hr2); eauto.
+      { admit.
+        (* destruct (decide (r2 = PC)) as [Heq|Heq]; simplify_map_eq. *)
+        (* - rewrite (fixpoint_interp1_eq _ (WCap p g b e a)) /=. *)
+        (*   destruct Hp as [Hp | [Hp | [Hp Hg] ] ]; subst p; try subst g. *)
+        (*   all: iApply (big_sepL_mono with "Hinv_interp"). *)
+        (*   all: intros; iIntros "H"; simpl. *)
+        (*   all: try( iDestruct "H" *)
+        (*            as (p P' Hfl HpersP') "(Hrel & Hzcond & Hrcond & Hwcond & HmonoR & %Hstate)"). *)
+        (*   all: iExists p,P'; iFrame "%∗". *)
+        (* - unshelve iSpecialize ("Hreg" $! r2 _ _ Hr2); eauto. *)
       }
 
       iApply wp_pure_step_later; auto; iNext; iIntros "_".
@@ -102,7 +103,7 @@ Section fundamental.
           iApply (sealing_preserves_interp with "[HVsb HVsr]"); eauto.
         }
         { by iApply "Hreg". }
-      + iApply (interp_next_PC with "IH Hinv_interp"); eauto.
-  Qed.
+      + iApply (interp_next_PC with "Hinv_interp"); eauto.
+  Admitted.
 
 End fundamental.
